AutomataTheory/Automata/OI2.lean
@@ -126,8 +126,8 @@ private lemma automata_oi2_lemma2 {as : ℕ → A} {ss : ℕ → (Automaton.OI2 
     assumption
 
 theorem accepted_omega_lang_inter2 :
-    AcceptedOmegaLang (Automaton.OI2 M acc) (Automaton.OI2_Acc M acc) = ⋂ i : Fin 2, AcceptedOmegaLang (M i) (acc i) := by
-  ext as ; simp [AcceptedOmegaLang, BuchiAccept]
+    (Automaton.OI2 M acc).AcceptedOmegaLang (Automaton.OI2_Acc M acc) = ⋂ i : Fin 2, (M i).AcceptedOmegaLang (acc i) := by
+  ext as ; simp [Automaton.AcceptedOmegaLang, BuchiAccept]
   constructor
   · rintro ⟨ss, h_run, h_inf⟩ i
     have h_run1 := automata_hist_inf_run_proj h_run
